MakeSetReader extern and Java implementation

Source/DafnyStandardLibraries/src/Std/ActionsExterns/IteratorAsProducer.java
@@ -1,0 +1,43 @@
+/*******************************************************************************
+*  Copyright by the contributors to the Dafny Project
+*  SPDX-License-Identifier: MIT
+*******************************************************************************/
+
+package Std.ActionsExterns;
+
+import java.util.Iterator;
+
+import Std.Producers.Producer;
+import Std.Producers._Companion_Producer;
+import Std.Wrappers.Option;
+
+import dafny.Tuple0;
+import dafny.TypeDescriptor;
+
+class IteratorAsProducer<T> implements Producer<T> {
+    private final TypeDescriptor td;
+    private final Iterator<? extends T> iterator;
+
+    public IteratorAsProducer(TypeDescriptor td, java.util.Iterator<? extends T> iterator) {
+        this.td = td;
+        this.iterator = iterator;
+    }
+
+    @Override
+    public Option<T> Invoke(Tuple0 i) {
+        if (iterator.hasNext()) {
+          return Option.create_Some(td, iterator.next());
+        } else {
+          return Option.create_None(td);
+        }
+    }
+
+    public void ForEachRemaining(Std.Consumers.IConsumer<T> consumer) {
+      _Companion_Producer.ForEachRemaining(td, this, consumer);
+    }
+
+    public Option<T> Next() {
+      return _Companion_Producer.Next(td, this);
+    }
+  
+}
