Source/DafnyStandardLibraries/src/Std/ActionsExterns/ProducerAsIterator.java
@@ -1,0 +1,39 @@
+/*******************************************************************************
+*  Copyright by the contributors to the Dafny Project
+*  SPDX-License-Identifier: MIT
+*******************************************************************************/
+
+package Std.ActionsExterns;
+
+import java.util.Iterator;
+
+import Std.Producers.Producer;
+import Std.Wrappers.Option;
+
+import dafny.Tuple0;
+
+class ProducerAsIterator<T> implements Iterator<T> {
+    private final Producer<T> producer;
+    private Option<T> next;
+
+    public ProducerAsIterator(Producer<T> producer) {
+        this.producer = producer;
+        fetchNext();
+    }
+
+    @Override
+    public boolean hasNext() {
+        return next.is_Some();
+    }
+
+    @Override
+    public T next() {
+        T result = next.dtor_value();
+        fetchNext();
+        return result;
+    }
+
+    private void fetchNext() {
+      this.next = producer.Invoke(Tuple0.create());
+    }
+}
