Source/DafnyStandardLibraries/src/Std/TargetSpecific/ActionsExterns-notarget-java.dfy
@@ -1,0 +1,9 @@
+/*******************************************************************************
+ *  Copyright by the contributors to the Dafny Project
+ *  SPDX-License-Identifier: MIT
+ *******************************************************************************/
+
+module {:extern} Std.JavaActionsExterns replaces ActionsExterns {
+
+  method {:extern} {:axiom} MakeSetReader<T>(s: set<T>) returns (p: Producer<T>, ghost proof: ProducerOfSetProof<T>)
+}
